src/cbor/spec/raw/CBOR.Spec.Raw.fst
@@ -106,9 +106,6 @@ let mk_det_raw_cbor c =
 
 let rec no_repeats_map_fst_mk_det_raw_cbor_map_entry
   (l: list (cbor & cbor))
-: Lemma
-  (requires (List.Tot.no_repeats_p (List.Tot.map fst l)))
-  (ensures (List.Tot.no_repeats_p (List.Tot.map fst (List.Tot.map mk_det_raw_cbor_map_entry l))))
 = match l with
   | [] -> ()
   | a :: q ->
